src/Init/Data/Char/Lemmas.lean
@@ -69,4 +69,9 @@ def notLTTotal : Std.Total (¬ · < · : Char → Char → Prop) where
   rw [Char.ofNat, dif_pos]
   rfl
 
+@[simp]
+theorem toUInt8_val {c : Char} : c.val.toUInt8 = c.toUInt8 := rfl
+
+theorem toString_eq_singleton {c : Char} : c.toString = String.singleton c := rfl
+
 end Char
